ironfleet/src/Dafny/Distributed/Protocol/ZooKeeper/PerformamceProof/ProofEmptyDiff_Invariants.dfy
@@ -14,6 +14,7 @@ include "Definitions.dfy"
 include "PerformancePredicates.dfy"
 include "ProtocolInvariants.dfy"
 include "Commons.dfy"
+include "EmptyDiffInvariants.dfy"
 
 
 module Zookeeper_PerformanceProof_Invariants {
@@ -32,7 +33,7 @@ import opened ZooKeeper_TimestampedDistributedSystem
 import opened Zookeeper_PerformancePredicates
 import opened Zookeeper_ProtocoIInvariants
 import opened Zookeeper_Commons
-
+import opened Zookeeper_EmptyDiffInvariants
 
 
 /*****************************************************************************************
@@ -272,6 +273,7 @@ lemma lemma_Leader_ProcessAck_PreQuorum_Invariant_Induction(config:Config, tls:T
     requires General_LS_Performance_Assumption(tls)
     requires Basic_Invariants(config, tls) && Basic_Invariants(config, tls')
     requires EmptyDiff_Invariant(tls) && EmptyDiff_Invariant(tls')
+    requires Handshake_Follower_Invariant(tls) && Handshake_Follower_Invariant(tls')
     // requires FollowerInit_Invariant(tls) && FollowerInit_Invariant(tls')
     // requires QuorumsMonotoneIncreasing_Property(tls, tls')
     // Induction hypothesis
@@ -284,29 +286,37 @@ lemma lemma_Leader_ProcessAck_PreQuorum_Invariant_Induction(config:Config, tls:T
 {
     var f, n := tls.f, |tls.config|;
 
-    // TODO
-    assume Sync_Follower_Invariant(tls');
+    // Prove Sync_Follower_Invariant(tls')
+    forall ep | 
+        && ep in tls'.t_servers
+        && tls'.t_servers[ep].v.FollowerPeer? 
+        && tls'.t_servers[ep].v.follower.state == F_SYNC
+        && 0 <= tls'.t_servers[ep].v.follower.serialSync < tls'.f
+    ensures && tls'.t_servers[ep].dts <= Follower_F_SYNC_dts_Formula(tls'.f, tls'.t_servers[ep])
+            && tls'.t_servers[ep].ts <= Follower_F_SYNC_ts_Formula(tls'.f, tls'.t_servers[ep])
+    {
+        Sync_Messages_Invariant_Helper_D(config, tls, tls', ep);
+    }
+    assert Sync_Follower_Invariant(tls');
 
     // Prove Sync_Messages_Invariant(tls');
     forall pkt | pkt in tls'.t_environment.sentPackets && (pkt.msg.v.SyncDIFF? || pkt.msg.v.SyncSNAP?)
-    ensures pkt.msg.ts <= Sync_Message_ts_Formula(f, pkt.msg.v.serial)
-    {
+    ensures pkt.msg.ts <= Sync_Message_ts_Formula(f, pkt.msg.v.serial) {
         assert pkt.msg.v.SyncDIFF?;  // By EmptyDiff_Invariant
         Sync_Messages_Invariant_Helper_A(config, tls, tls', pkt);
     }
     forall pkt | pkt in tls'.t_environment.sentPackets && pkt.msg.v.NewLeader?
-    ensures pkt.msg.ts <= NewLeader_Message_ts_Formula(tls.f, pkt.msg.v.serial)
-    {
+    ensures pkt.msg.ts <= NewLeader_Message_ts_Formula(tls.f, pkt.msg.v.serial) {
         Sync_Messages_Invariant_Helper_B(config, tls, tls', pkt);
     }
 
     forall pkt | pkt in tls'.t_environment.sentPackets && pkt.msg.v.Ack?
-    ensures pkt.msg.ts <= Ack_Message_ts_Formula(tls.f, pkt.msg.v.serial)
-    {
+    ensures pkt.msg.ts <= Ack_Message_ts_Formula(tls.f, pkt.msg.v.serial) {
         Sync_Messages_Invariant_Helper_C(config, tls, tls', pkt);
     }
-
     assert Sync_Messages_Invariant(tls');
+
+    // Prove Sync_Leader_PreQuorum_Invariant(tls')
     assume Sync_Leader_PreQuorum_Invariant(tls');
 }
 
@@ -383,8 +393,70 @@ lemma Sync_Messages_Invariant_Helper_C(config:Config, tls:TLS_State, tls':TLS_St
     var f, n := tls.f, |tls.config|;
     if pkt !in tls.t_environment.sentPackets {
         var actor, tios:seq<TZKIo> :| actor in tls.t_servers && TLS_NextOneServer(tls, tls', actor, tios);
-        assert tls.t_servers[actor].v.follower.serialSync >= 0;
+        assert tls'.t_servers[actor].v.follower.serialSync >= 0;
         assert pkt.msg.ts <= Ack_Message_ts_Formula(f, pkt.msg.v.serial);
+    }
+}
+
+lemma Sync_Messages_Invariant_Helper_D(config:Config, tls:TLS_State, tls':TLS_State, ep:EndPoint) 
+    requires TLS_Next(tls, tls')
+    requires General_LS_Performance_Assumption(tls)
+    requires Basic_Invariants(config, tls) && Basic_Invariants(config, tls')
+    requires EmptyDiff_Invariant(tls) && EmptyDiff_Invariant(tls')
+    requires Handshake_Follower_Invariant(tls) && Handshake_Follower_Invariant(tls')
+    // Induction hypothesis
+    requires Sync_Messages_Invariant(tls)
+    requires Sync_Follower_Invariant(tls)
+    requires Sync_Leader_PreQuorum_Invariant(tls)
+    // Antecedent
+    requires ep in tls'.t_servers
+    requires tls'.t_servers[ep].v.FollowerPeer? 
+    requires tls'.t_servers[ep].v.follower.state == F_SYNC
+    requires 0 <= tls'.t_servers[ep].v.follower.serialSync < tls'.f
+    // Conclusion
+    ensures tls'.t_servers[ep].dts <= Follower_F_SYNC_dts_Formula(tls'.f, tls'.t_servers[ep])
+    ensures tls'.t_servers[ep].ts <= Follower_F_SYNC_ts_Formula(tls'.f, tls'.t_servers[ep])
+{
+    var f, n := tls.f, |tls.config|;
+    var actor, tios:seq<TZKIo> :| actor in tls.t_servers && TLS_NextOneServer(tls, tls', actor, tios);
+    var ls, ls', ios := UntagLS_State(tls), UntagLS_State(tls'), UntagLIoOpSeq(tios);
+    if actor != ep {return;}
+    var s, s' := ls.servers[actor].follower, ls'.servers[actor].follower;
+    var st, st' := tls.t_servers[actor], tls'.t_servers[actor];
+    var pkt := tios[0].r;
+    
+    // s can be in two possible states. 1) F_PRESYNC, 2) F_SYNC
+    if s.state == F_PRESYNC {
+        assert pkt.msg.v.SyncDIFF?;
+        assert st'.dts <= Follower_F_SYNC_dts_Formula(f, st');
+        assert st.ts <= LeaderInfo_Message_PreQuorum_ts_Formula(f, s.serialLI) + ProcLI;
+        assert pkt.msg.ts <= Sync_Message_ts_Formula(f, pkt.msg.v.serial);
+        assert s'.state == F_SYNC;
+        var handlerStartTime := TimeMax(st.ts, pkt.msg.ts);
+        lemma_Math_Inequalities_CommonMult(ProcFI, s.serialLI+1, f);
+        lemma_Math_MaxOfInequalities(st.ts, pkt.msg.ts, 
+        LeaderInfo_Message_PreQuorum_ts_Formula(f, s.serialLI) + ProcLI, 
+        Sync_Message_ts_Formula(f, pkt.msg.v.serial));
+        assert st'.ts <= Follower_F_SYNC_ts_Formula(f, st');
+    } else {
+        assert s.state == F_SYNC;
+        assert st'.dts <= Follower_F_SYNC_dts_Formula(f, st');
+        assert pkt.msg.v.NewLeader?;
+        lemma_Math_Inequalities_CommonMult(Sync, s.serialSync, f);
+        lemma_Math_Inequalities_CommonMult(Sync, s.serialSync + 1, f);
+        lemma_Math_Inequalities_CommonMult(Sync, s.serialSync, f);
+        lemma_Math_Inequalities_CommonMult(Sync, s.serialSync + 1, f);
+        lemma_Math_Inequalities_CommonMult(Sync, pkt.msg.v.serial + 1, f);
+        var handlerStartTime := TimeMax(st.ts, pkt.msg.ts);
+        lemma_Math_MaxOfInequalities(pkt.msg.ts, st.ts, 
+        NewLeader_Message_ts_Formula(f, pkt.msg.v.serial), 
+        AckEpoch_Message_PreQuorum_ts_Formula(f, f-1)
+            + PreSync * f    
+            + Sync * f  
+            + Sync * f  
+            + D
+            + ProcSyncI);      
+        assert st'.ts <= Follower_F_SYNC_ts_Formula(f, st');
     }
 }
 
